Make computability/lambda/churchpair look modern and pretty

examples/computability/lambda/churchpairScript.sml
@@ -10,145 +10,144 @@ open reductionEval
 
 val _ = new_theory "churchpair"
 
-val _ = set_trace "Unicode" 1
-
-fun Store_thm(n,t,tac) = store_thm(n,t,tac) before export_rewrites [n]
-
-val cvpr_def = Define`
+Definition cvpr_def:
   cvpr M N = let v = NEW (FV M ∪ FV N)
              in
                LAM v (VAR v @@ M @@ N)
-`;
+End
 
-val FV_cvpr = Store_thm(
-  "FV_cvpr",
-  ``FV (cvpr M N) = FV M ∪ FV N``,
+Theorem FV_cvpr[simp]:
+  FV (cvpr M N) = FV M ∪ FV N
+Proof
   SRW_TAC [][cvpr_def, EXTENSION, LET_THM] THEN
-  NEW_ELIM_TAC THEN METIS_TAC []);
-val bnf_cvpr = Store_thm(
-  "bnf_cvpr",
-  ``bnf (cvpr M N) <=> bnf M ∧ bnf N``,
-  SRW_TAC [][cvpr_def, LET_THM]);
+  NEW_ELIM_TAC THEN METIS_TAC []
+QED
 
-val cvpr_fresh = store_thm(
-  "cvpr_fresh",
-  ``v ∉ FV M ∧ v ∉ FV N ⇒ (cvpr M N = LAM v (VAR v @@ M @@ N))``,
+Theorem bnf_cvpr[simp]:
+  bnf (cvpr M N) ⇔ bnf M ∧ bnf N
+Proof SRW_TAC [][cvpr_def, LET_THM]
+QED
+
+Theorem cvpr_fresh:
+  v ∉ FV M ∧ v ∉ FV N ⇒ cvpr M N = LAM v (VAR v @@ M @@ N)
+Proof
   SRW_TAC [][LET_THM, cvpr_def] THEN NEW_ELIM_TAC THEN
-  SRW_TAC [][LAM_eq_thm, tpm_fresh]);
+  SRW_TAC [][LAM_eq_thm, tpm_fresh]
+QED
 
-val cvpr_11 = Store_thm(
-  "cvpr_11",
-  ``cvpr M₁ N₁ = cvpr M₂ N₂ <=> M₁ = M₂ ∧ N₁ = N₂``,
-  Q_TAC (NEW_TAC "z") `FV M₁ ∪ FV M₂ ∪ FV N₁ ∪ FV N₂` THEN
-  `(cvpr M₁ N₁ = LAM z (VAR z @@ M₁ @@ N₁)) ∧
-   (cvpr M₂ N₂ = LAM z (VAR z @@ M₂ @@ N₂))`
+Theorem cvpr_11[simp]:
+  cvpr M₁ N₁ = cvpr M₂ N₂ ⇔ M₁ = M₂ ∧ N₁ = N₂
+Proof
+  Q_TAC (NEW_TAC "z") ‘FV M₁ ∪ FV M₂ ∪ FV N₁ ∪ FV N₂’ THEN
+  ‘(cvpr M₁ N₁ = LAM z (VAR z @@ M₁ @@ N₁)) ∧
+   (cvpr M₂ N₂ = LAM z (VAR z @@ M₂ @@ N₂))’
      by SRW_TAC [][cvpr_fresh] THEN
-  SRW_TAC [][]);
+  SRW_TAC [][]
+QED
 
-val SUB_cvpr = Store_thm(
-  "SUB_cvpr",
-  ``[M/v] (cvpr N P) = cvpr ([M/v]N) ([M/v]P)``,
-  Q_TAC (NEW_TAC "z") `{v} ∪ FV M ∪ FV N ∪ FV P` THEN
-  `z ∉ FV ([M/v]N) ∧ z ∉ FV ([M/v]P)`
-     by SRW_TAC [][termTheory.FV_SUB] THEN
-  `(cvpr N P = LAM z (VAR z @@ N @@ P)) ∧
-   (cvpr ([M/v]N) ([M/v]P) = LAM z (VAR z @@ [M/v]N @@ [M/v]P))`
+Theorem SUB_cvpr[simp]:
+  [M/v] (cvpr N P) = cvpr ([M/v]N) ([M/v]P)
+Proof
+  Q_TAC (NEW_TAC "z") ‘{v} ∪ FV M ∪ FV N ∪ FV P’ THEN
+  ‘z ∉ FV ([M/v]N) ∧ z ∉ FV ([M/v]P)’ by SRW_TAC [][termTheory.FV_SUB] THEN
+  ‘(cvpr N P = LAM z (VAR z @@ N @@ P)) ∧
+   (cvpr ([M/v]N) ([M/v]P) = LAM z (VAR z @@ [M/v]N @@ [M/v]P))’
      by SRW_TAC [][cvpr_fresh] THEN
-  SRW_TAC [][]);
-val tpm_cvpr = Store_thm(
-  "tpm_cvpr",
-  ``tpm pi (cvpr x y) = cvpr (tpm pi x) (tpm pi y)``,
+  SRW_TAC [][]
+QED
+Theorem tpm_cvpr[simp]:
+  tpm pi (cvpr x y) = cvpr (tpm pi x) (tpm pi y)
+Proof
   SRW_TAC [][cvpr_def, LET_THM] THEN
   NTAC 2 (NEW_ELIM_TAC THEN SRW_TAC [][]) THEN
   SRW_TAC [CONJ_ss][LAM_eq_thm] THEN
-  Cases_on `lswapstr pi v = v'` THEN SRW_TAC [][] THEN
+  Cases_on ‘lswapstr pi v = v'’ THEN SRW_TAC [][] THEN
   ONCE_REWRITE_TAC [EQ_SYM_EQ] THEN
-  MATCH_MP_TAC tpm_fresh THEN SRW_TAC [][]);
+  MATCH_MP_TAC tpm_fresh THEN SRW_TAC [][]
+QED
 
-val cpair_def = Define`
+Definition cpair_def:
   cpair = LAM "x" (LAM "y" (LAM "f" (VAR "f" @@ VAR "x" @@ VAR "y")))
-`;
+End
 
-val FV_cpair = Store_thm(
-  "FV_cpair",
-  ``FV cpair = {}``,
-  SRW_TAC [][cpair_def, EXTENSION] THEN METIS_TAC []);
-val bnf_cpair = Store_thm(
-  "bnf_cpair",
-  ``bnf cpair``,
-  SRW_TAC [][cpair_def]);
-val cpair_behaviour = store_thm(
-  "cpair_behaviour",
-  ``cpair @@ M @@ N -n->* cvpr M N``,
+Theorem FV_cpair[simp]:    FV cpair = {}
+Proof    SRW_TAC [][cpair_def, EXTENSION] THEN METIS_TAC []
+QED
+
+Theorem bnf_cpair[simp]:   bnf cpair
+Proof    SRW_TAC [][cpair_def]
+QED
+
+Theorem cpair_behaviour:
+  cpair @@ M @@ N -n->* cvpr M N
+Proof
   SRW_TAC [][cpair_def] THEN FRESH_TAC THEN
   MP_TAC (Q.GEN `M` (Q.GEN `N` (Q.INST [`v` |-> `f`] cvpr_fresh))) THEN
-  SRW_TAC [][] THEN
-  SRW_TAC [NORMSTAR_ss][]);
+  SRW_TAC [][] THEN SRW_TAC [NORMSTAR_ss][]
+QED
 
-val wh_cpair = store_thm(
-  "wh_cpair",
-  ``cpair @@ x @@ y @@ f -w->* f @@ x @@ y``,
+Theorem wh_cpair:
+  cpair @@ x @@ y @@ f -w->* f @@ x @@ y
+Proof
   REWRITE_TAC [cpair_def] THEN
   unvarify_tac head_reductionTheory.whstar_substitutive THEN
-  ASM_SIMP_TAC (whfy (srw_ss())) []);
+  ASM_SIMP_TAC (whfy (srw_ss())) []
+QED
 
-
-
-val cfst_def = Define`
+Definition cfst_def:
   cfst = LAM "p" (VAR "p" @@ cB T)
-`;
-val FV_cfst = Store_thm(
-  "FV_cfst",
-  ``FV cfst = {}``,
-  SRW_TAC [][cfst_def])
-val bnf_cfst = Store_thm(
-  "bnf_cfst",
-  ``bnf cfst``,
-  SRW_TAC [][cfst_def]);
+End
+Theorem FV_cfst[simp]:     FV cfst = {}
+Proof SRW_TAC [][cfst_def]
+QED
+Theorem bnf_cfst[simp]:    bnf cfst
+Proof SRW_TAC [][cfst_def]
+QED
 
-val csnd_def = Define`
+Definition csnd_def:
   csnd = LAM "p" (VAR "p" @@ cB F)
-`;
-val FV_csnd = Store_thm(
-  "FV_csnd",
-  ``FV csnd = {}``,
-  SRW_TAC [][csnd_def])
-val bnf_csnd = Store_thm(
-  "bnf_csnd",
-  ``bnf csnd``,
-  SRW_TAC [][csnd_def]);
+End
+Theorem FV_csnd[simp]:     FV csnd = {}
+Proof SRW_TAC [][csnd_def]
+QED
+Theorem bnf_csnd[simp]:    bnf csnd
+Proof SRW_TAC [][csnd_def]
+QED
 
-val is_abs_cfstsnd = Store_thm(
-  "is_abs_cfstsnd",
-  ``is_abs csnd ∧ is_abs cfst``,
-  SRW_TAC [][cfst_def, csnd_def]);
+Theorem is_abs_cfstsnd[simp]:    is_abs csnd ∧ is_abs cfst
+Proof SRW_TAC [][cfst_def, csnd_def]
+QED
 
-val cfst_pair = store_thm(
-  "cfst_pair",
-  ``cfst @@ (cpair @@ M @@ N) -n->* M``,
+Theorem cfst_pair:
+  cfst @@ (cpair @@ M @@ N) -n->* M
+Proof
   SRW_TAC [][cfst_def, cpair_def] THEN FRESH_TAC THEN
-  SRW_TAC [NORMSTAR_ss][tpm_fresh, cB_behaviour]);
+  SRW_TAC [NORMSTAR_ss][tpm_fresh, cB_behaviour]
+QED
 val _ = export_betarwt "cfst_pair"
 
-val csnd_pair = store_thm(
-  "csnd_pair",
-  ``csnd @@ (cpair @@ M @@ N) -n->* N``,
+Theorem csnd_pair:
+  csnd @@ (cpair @@ M @@ N) -n->* N
+Proof
   SRW_TAC [][csnd_def, cpair_def] THEN FRESH_TAC THEN
-  SRW_TAC [NORMSTAR_ss][tpm_fresh, cB_behaviour])
+  SRW_TAC [NORMSTAR_ss][tpm_fresh, cB_behaviour]
+QED
 val _ = export_betarwt "csnd_pair"
 
-val cfst_cvpr = store_thm(
-  "cfst_cvpr",
-  ``cfst @@ cvpr M N -n->* M``,
+Theorem cfst_cvpr:
+  cfst @@ cvpr M N -n->* M
+Proof
   SRW_TAC [][cfst_def, cvpr_def, LET_THM] THEN NEW_ELIM_TAC THEN
-  SRW_TAC [NORMSTAR_ss][cB_behaviour]);
+  SRW_TAC [NORMSTAR_ss][cB_behaviour]
+QED
 val _ = export_betarwt "cfst_cvpr"
 
-val csnd_cvpr = store_thm(
-  "csnd_cvpr",
-  ``csnd @@ cvpr M N -n->* N``,
+Theorem csnd_cvpr:
+  csnd @@ cvpr M N -n->* N
+Proof
   SRW_TAC [][csnd_def, cvpr_def, LET_THM] THEN NEW_ELIM_TAC THEN
-  SRW_TAC [NORMSTAR_ss][cB_behaviour]);
+  SRW_TAC [NORMSTAR_ss][cB_behaviour]
+QED
 val _ = export_betarwt "csnd_cvpr"
 
 val _ = export_theory()
